linking/sepcomp.v
@@ -6,6 +6,7 @@ Require Export sepcomp.StructuredInjections.
 Require Export sepcomp.effect_semantics.
 Require Export sepcomp.reach. 
 Require Export sepcomp.effect_simulationsEXP.
+Require Export sepcomp.wholeprog_simulations.
 Require Export sepcomp.effect_properties.
 Require Export sepcomp.step_lemmas.
 Require Export sepcomp.extspec.
